Finish Abs_Int_C locale

Uppaal_Networks/AbsInt/AbsInt_Instrc.thy
@@ -5,34 +5,38 @@ begin
 definition extract_prog :: "'t programc \<Rightarrow> program" where
   "extract_prog p = (\<lambda>cop. case cop of Some (INSTR op) \<Rightarrow> Some op | Some (CEXP _) \<Rightarrow> Some NOP | None \<Rightarrow> None) \<circ> p"
 
-fun astep_liftc :: "'a::absstate astep \<Rightarrow> 't programc \<Rightarrow> instr \<Rightarrow> addr \<Rightarrow> 'a \<Rightarrow> 'a state_map" where
-  "astep_liftc f prog op pc s =
+fun astep_liftc :: "'a::absstate astep \<Rightarrow> ('a \<Rightarrow> 'a) \<Rightarrow> 't programc \<Rightarrow> instr \<Rightarrow> addr \<Rightarrow> 'a \<Rightarrow> 'a state_map" where
+  "astep_liftc f kill_flag prog op pc s =
     (case prog pc of
-      (Some (CEXP _)) \<Rightarrow> (if s = \<bottom> then \<bottom> else undefined) |
+      (Some (CEXP _)) \<Rightarrow> (if s = \<bottom> then \<bottom> else single (Suc pc) (kill_flag s)) |
       _ \<Rightarrow> f op pc s)"
 
 lemma astep_liftc_keep_bot:
   assumes "lookup (f op ipc \<bottom>) pc = \<bottom>"
-  shows "lookup (astep_liftc f prog op ipc \<bottom>) pc = \<bottom>"
+  shows "lookup (astep_liftc f kf prog op ipc \<bottom>) pc = \<bottom>"
 using assms proof (cases "prog ipc")
   case (Some cop)
   then show ?thesis using assms by (cases cop; simp)
 qed simp
 
-context Abs_Int
+locale Abs_Int_C = Abs_Int +
+  fixes kill_flag :: "'a \<Rightarrow> 'a"
+  assumes kill_flag: "(st, s, f, rs) \<in> \<gamma> x \<Longrightarrow> (st, s, True, rs) \<in> \<gamma> (kill_flag x) \<and> (st, s, False, rs) \<in> \<gamma> (kill_flag x)"
 begin
 
+abbreviation "astepc \<equiv> astep_liftc ai_step kill_flag"
+
 lemma astep_liftc_keep_bot_map:
-  "astep_liftc ai_step prog op ipc \<bottom> = \<bottom>"
+  "astepc prog op ipc \<bottom> = \<bottom>"
 proof (rule state_map_eq_fwd, goal_cases)
   case (1 p)
-  have "lookup (astep_liftc ai_step prog op ipc \<bottom>) p = \<bottom>"
+  have "lookup (astepc prog op ipc \<bottom>) p = \<bottom>"
     using astep_keep_bot by (rule astep_liftc_keep_bot)
   also have "\<dots> = lookup \<bottom> p" by simp
   finally show ?case .
 qed
 
-definition "ai_loopc cprog \<equiv> finite_loop (astep_liftc ai_step cprog) (extract_prog cprog)"
+definition "ai_loopc cprog \<equiv> finite_loop (astepc cprog) (extract_prog cprog)"
 
 theorem ai_stepsc:
   assumes "stepsc cprog (Suc n) u (pc, st, s, f, rs) (pc', st', s', f', rs')"
@@ -56,10 +60,10 @@ next
     then obtain pc'' st'' s'' f'' rs'' where inter: "inter = (pc'', st'', s'', f'', rs'')"
       using state_pc.cases by blast
     let ?anter = "ai_loopc cprog 1 entry"
-    have "(st'', s'', f'', rs'') \<in> \<gamma> (lookup (finite_step_map (astep_liftc ai_step cprog) (extract_prog cprog) entry) pc'')"
+    have in_step_map: "(st'', s'', f'', rs'') \<in> \<gamma> (lookup (finite_step_map (astepc cprog) (extract_prog cprog) entry) pc'')"
     proof (cases cmd)
       case (INSTR instr)
-      hence same: "astep_liftc ai_step cprog instr pc (lookup entry pc) = ai_step instr pc (lookup entry pc)" using 2 by simp
+      hence same: "astepc cprog instr pc (lookup entry pc) = ai_step instr pc (lookup entry pc)" using 2 by simp
       have "(st'', s'', f'', rs'') \<in> \<gamma> (lookup (ai_step instr pc (lookup entry pc)) pc'')"
       proof -
         from \<open>stepc _ _ _ = _\<close> have "UPPAAL_Asm.step instr (pc, st, s, f, rs) = Some (pc'', st'', s'', f'', rs'')"
@@ -68,8 +72,8 @@ next
           using Suc.prems(2) by auto
         thus ?thesis using astep_correct by blast
       qed
-      hence "(st'', s'', f'', rs'') \<in> \<gamma> (lookup ((astep_liftc ai_step cprog) instr pc (lookup entry pc)) pc'')" using same by simp
-      moreover have "astep_liftc ai_step cprog instr pc (lookup entry pc) \<le> finite_step_map (astep_liftc ai_step cprog) (extract_prog cprog) entry"
+      hence "(st'', s'', f'', rs'') \<in> \<gamma> (lookup (astepc cprog instr pc (lookup entry pc)) pc'')" using same by simp
+      moreover have "astepc cprog instr pc (lookup entry pc) \<le> finite_step_map (astepc cprog) (extract_prog cprog) entry"
       proof -
         have "(extract_prog cprog) pc = Some instr" unfolding extract_prog_def using 2 INSTR by simp
         then show ?thesis using calculation astep_liftc_keep_bot_map finite_step_map_step by blast
@@ -77,12 +81,23 @@ next
       ultimately show ?thesis using less_eq_state_map_def mono_gamma by blast
     next
       case (CEXP x2)
-      then show ?thesis sorry
+      then have out: "pc'' = Suc pc \<and> st'' = st \<and> s'' = s \<and> rs'' = rs" using "2"(1) inter by simp
+      hence "(st'', s'', f'', rs'') \<in> \<gamma> (kill_flag (lookup entry pc))" using out
+        by (metis (full_types) Suc.prems(2) kill_flag)
+      hence "(st'', s'', f'', rs'') \<in> \<gamma> (lookup (single (Suc pc) (kill_flag (lookup entry pc))) pc'')" using out by simp
+      hence "(st'', s'', f'', rs'') \<in> \<gamma> (lookup (astepc cprog NOP pc (lookup entry pc)) pc'')"
+        using CEXP 2 Suc.prems by auto
+      moreover have "astepc cprog NOP pc (lookup entry pc) \<le> finite_step_map (astepc cprog) (extract_prog cprog) entry"
+      proof -
+        have "(extract_prog cprog) pc = Some NOP" unfolding extract_prog_def using 2 CEXP by simp
+        then show ?thesis using calculation astep_liftc_keep_bot_map finite_step_map_step by blast
+      qed
+      ultimately show ?thesis using less_eq_state_map_def mono_gamma by blast
     qed
-    hence "(st'', s'', f'', rs'') \<in> \<gamma> (lookup (finite_advance (astep_liftc ai_step cprog) (extract_prog cprog) entry) pc'')"
-      by (metis (no_types, lifting) finite_advance.elims le_sup_iff less_eq_state_map_def mono_gamma order_refl subsetD)
-    hence "(st'', s'', f'', rs'') \<in> \<gamma> (lookup ?anter pc'')" by (simp add: ai_loopc_def)
-    then show ?thesis using Suc.IH by (metis (no_types, lifting) "2"(3) One_nat_def inter ai_loopc_def finite_loop.simps(1) finite_loop.simps(2))
+    moreover have "finite_step_map (astepc cprog) (extract_prog cprog) entry \<le> finite_advance (astepc cprog) (extract_prog cprog) entry" by simp
+    ultimately have "(st'', s'', f'', rs'') \<in> \<gamma> (lookup (finite_advance (astepc cprog) (extract_prog cprog) entry) pc'')"
+      using less_eq_state_map_def mono_gamma by blast
+    then show ?thesis using Suc.IH by (metis "2"(3) ai_loopc_def finite_loop.simps(2) inter)
   qed
 qed
 
